Building up the Fragmenta github repository

Isabelle/INTO-CPS/INTO_SysML_3WTs_loop.thy
@@ -3,15 +3,15 @@
     Author:     Nuno Amálio
 *)
 
-theory INTO_SysML_3WTs
+theory INTO_SysML_3WTs_loop
 imports INTO_SysML_MM_Gbl PDGs
   
 begin
 
 (*The ASD corresponding to the ASD of 3WTs*)
-definition SG_ASD_3WTs :: "SGr_ls"
+definition SG_ASD_3WTs_loop :: "SGr_ls"
 where
-  "SG_ASD_3WTs = \<lparr>NsG=[''WaterTanksASD'', ''WaterTanksSys'', ''CompWaterTanksSys1'',
+  "SG_ASD_3WTs_loop = \<lparr>NsG=[''WaterTanksASD'', ''WaterTanksSys'', ''CompWaterTanksSys1'',
     ''CompWaterTanksSys2'', ''CompWaterTanksSys3'',
     ''TanksControl1'', 
     ''TanksControl2'', ''CompTanksControl1Valve'', ''CompTanksControl1WaterTank'', 
@@ -19,7 +19,7 @@ where
     ''Controller'',
     ''Valve'', ''WaterTank'', ''FlowRate'', ''Area'', ''Height'', ''OpenClosed'',
     ''WaterTank_win'', ''WaterTank_wout'', ''Valve_v2'', ''Valve_w'', 
-    ''Controller_v1''], 
+    ''Controller_v1'', ''Controller_win''], 
       EsG = [''EWaterTanksASD_WaterTanksSys'', ''EWaterTanksASD_TanksControl1'', 
         ''EWaterTanksASD_TanksControl2'', ''EWaterTanksASD_Valve'', 
         ''EWaterTanksASD_WaterTank'', ''EWaterTanksASD_FlowRate'', 
@@ -37,8 +37,8 @@ where
         ''ECompTanksControl1WaterTank_tgt'', 
         ''ECompTanksControl2WaterTank_tgt'', 
         ''E_WaterTank_win'', ''E_WaterTank_wout'', ''E_Valve_v2'', 
-        ''E_Valve_w'', ''E_Controller_v1'', ''E_Dep_w_v2'',
-        ''E_Dep_wout_win''], 
+        ''E_Valve_w'', ''E_Controller_v1'', ''E_Controller_win'', ''E_Dep_w_v2'',
+        ''E_Dep_wout_win'', ''E_Dep_v1_win''], 
       srcG =  [(''EWaterTanksASD_WaterTanksSys'', ''WaterTanksASD''), 
         (''EWaterTanksASD_TanksControl1'', ''WaterTanksASD''),
         (''EWaterTanksASD_TanksControl2'', ''WaterTanksASD''),
@@ -62,9 +62,10 @@ where
         (''ECompTanksControl2WaterTank_tgt'', ''CompTanksControl2WaterTank''),
         (''E_WaterTank_win'', ''WaterTank''), (''E_WaterTank_wout'', ''WaterTank''),
         (''E_Valve_v2'', ''Valve''), (''E_Valve_w'', ''Valve''), 
-        (''E_Controller_v1'', ''Controller''),
+        (''E_Controller_v1'', ''Controller''), (''E_Controller_win'', ''Controller''),
         (''E_Dep_w_v2'', ''Valve_w''), 
-        (''E_Dep_wout_win'', ''WaterTank_wout'')], 
+        (''E_Dep_wout_win'', ''WaterTank_wout''), 
+        (''E_Dep_v1_win'', ''Controller_v1'')], 
       tgtG =  [(''EWaterTanksASD_WaterTanksSys'', ''WaterTanksSys''), 
         (''EWaterTanksASD_TanksControl1'', ''TanksControl1''),
         (''EWaterTanksASD_TanksControl2'', ''TanksControl2''),
@@ -89,8 +90,10 @@ where
         (''E_WaterTank_win'', ''WaterTank_win''), 
         (''E_WaterTank_wout'', ''WaterTank_wout''),
         (''E_Valve_v2'', ''Valve_v2''), (''E_Valve_w'', ''Valve_w''), 
-        (''E_Controller_v1'', ''Controller_v1''),
-        (''E_Dep_w_v2'', ''Valve_v2''), (''E_Dep_wout_win'', ''WaterTank_win'')],
+        (''E_Controller_v1'', ''Controller_v1''), 
+        (''E_Controller_win'', ''Controller_win''),
+        (''E_Dep_w_v2'', ''Valve_v2''), (''E_Dep_wout_win'', ''WaterTank_win''),
+        (''E_Dep_v1_win'', ''Controller_win'')],
       ntyG =[(''WaterTanksASD'', nnrml), (''WaterTanksSys'',  nnrml), 
         (''CompWaterTanksSys1'', nnrml), (''CompWaterTanksSys2'', nnrml),
         (''CompWaterTanksSys3'', nnrml), (''CompTanksControl1Valve'', nnrml), 
@@ -104,7 +107,7 @@ where
         (''WaterTank_wout'', nnrml),
         (''Valve_v2'', nnrml), 
         (''Valve_w'', nnrml), 
-        (''Controller_v1'', nnrml)],
+        (''Controller_v1'', nnrml), (''Controller_win'', nnrml)],
       etyG =[(''EWaterTanksASD_WaterTanksSys'', elnk), 
         (''EWaterTanksASD_TanksControl1'', elnk),
         (''EWaterTanksASD_TanksControl2'', elnk),
@@ -130,8 +133,8 @@ where
         (''E_WaterTank_wout'', elnk),
         (''E_Valve_v2'', elnk), 
         (''E_Valve_w'', elnk), 
-        (''E_Controller_v1'', elnk), (''E_Dep_w_v2'', elnk),
-        (''E_Dep_wout_win'', elnk)],
+        (''E_Controller_v1'', elnk), (''E_Controller_win'', elnk), (''E_Dep_w_v2'', elnk),
+        (''E_Dep_wout_win'', elnk), (''E_Dep_v1_win'', elnk)],
       srcmG = [], 
       tgtmG = [(''ECompWaterTanksSys1_src'', sm (val 1)), 
         (''ECompWaterTanksSys2_src'', sm (val 1)), 
@@ -148,165 +151,168 @@ where
 
 axiomatization
 where
-  Es_SG_ASD_3WTs: "Es (toSGr SG_ASD_3WTs) \<subseteq> E_A"
-  and Ns_SG_ASD_3WTs: "Ns (toSGr SG_ASD_3WTs) \<subseteq> V_A"
+  Es_SG_ASD_3WTs_loop: "Es (toSGr SG_ASD_3WTs_loop) \<subseteq> E_A"
+  and Ns_SG_ASD_3WTs_loop: "Ns (toSGr SG_ASD_3WTs_loop) \<subseteq> V_A"
 
-value "consInh SG_ASD_3WTs"
+value "consInh SG_ASD_3WTs_loop"
 
-lemma wf_SG_ASD_3WTs: "is_wf_sg (toSGr SG_ASD_3WTs)"
+lemma wf_SG_ASD_3WTs_loop: "is_wf_sg (toSGr SG_ASD_3WTs_loop)"
   proof -
-    have h_wf_g: "is_wf_g (toSGr SG_ASD_3WTs)"
+    have h_wf_g: "is_wf_g (toSGr SG_ASD_3WTs_loop)"
       proof (simp add: is_wf_g_def, rule conjI)
-        show "Ns (toSGr SG_ASD_3WTs) \<subseteq> V_A"
-          using Ns_SG_ASD_3WTs by simp
+        show "Ns (toSGr SG_ASD_3WTs_loop) \<subseteq> V_A"
+          using Ns_SG_ASD_3WTs_loop by simp
       next
         apply_end(rule conjI)
-        show "Es (toSGr SG_ASD_3WTs) \<subseteq> E_A"
-          using Es_SG_ASD_3WTs by simp
+        show "Es (toSGr SG_ASD_3WTs_loop) \<subseteq> E_A"
+          using Es_SG_ASD_3WTs_loop by simp
       next
         apply_end(rule conjI)
-        show "ftotal_on (src (toSGr SG_ASD_3WTs)) (Es (toSGr SG_ASD_3WTs)) (Ns (toSGr SG_ASD_3WTs))"
-          by (simp add: ftotal_on_def toSGr_def SG_ASD_3WTs_def)
+        show "ftotal_on (src (toSGr SG_ASD_3WTs_loop)) (Es (toSGr SG_ASD_3WTs_loop)) (Ns (toSGr SG_ASD_3WTs_loop))"
+          by (simp add: ftotal_on_def toSGr_def SG_ASD_3WTs_loop_def)
       next
-        show "ftotal_on (tgt (toSGr SG_ASD_3WTs)) (Es (toSGr SG_ASD_3WTs)) (Ns (toSGr SG_ASD_3WTs))"
-          by (simp add: ftotal_on_def toSGr_def SG_ASD_3WTs_def)
+        show "ftotal_on (tgt (toSGr SG_ASD_3WTs_loop)) (Es (toSGr SG_ASD_3WTs_loop)) (Ns (toSGr SG_ASD_3WTs_loop))"
+          by (simp add: ftotal_on_def toSGr_def SG_ASD_3WTs_loop_def)
       qed
     show ?thesis
     proof (simp add: is_wf_sg_def, rule conjI)
-      show "is_wf_g (toSGr SG_ASD_3WTs)"
+      show "is_wf_g (toSGr SG_ASD_3WTs_loop)"
         using h_wf_g by simp
     next
       apply_end(rule conjI)
-      show "ftotal_on (nty (toSGr SG_ASD_3WTs)) (Ns (toSGr SG_ASD_3WTs)) SGNTy_set"
-        by (auto simp add: ftotal_on_def SGNTy_set_def SG_ASD_3WTs_def toSGr_def)
+      show "ftotal_on (nty (toSGr SG_ASD_3WTs_loop)) (Ns (toSGr SG_ASD_3WTs_loop)) SGNTy_set"
+        by (auto simp add: ftotal_on_def SGNTy_set_def SG_ASD_3WTs_loop_def toSGr_def)
     next
       apply_end(rule conjI) 
-      show "ftotal_on (ety (toSGr SG_ASD_3WTs)) (Es (toSGr SG_ASD_3WTs)) SGETy_set"
-        by (simp add: ftotal_on_def SGNTy_set_def SG_ASD_3WTs_def toSGr_def SGETy_set_def)
+      show "ftotal_on (ety (toSGr SG_ASD_3WTs_loop)) (Es (toSGr SG_ASD_3WTs_loop)) SGETy_set"
+        by (simp add: ftotal_on_def SGNTy_set_def SG_ASD_3WTs_loop_def toSGr_def SGETy_set_def)
     next
       apply_end(rule conjI) 
-      show "dom (srcm (toSGr SG_ASD_3WTs)) = EsTy (toSGr SG_ASD_3WTs) {Some erelbi, Some ecompbi}"
-        by (simp add: SG_ASD_3WTs_def toSGr_def EsTy_def vimage_def)
+      show "dom (srcm (toSGr SG_ASD_3WTs_loop)) = EsTy (toSGr SG_ASD_3WTs_loop) {Some erelbi, Some ecompbi}"
+        by (simp add: SG_ASD_3WTs_loop_def toSGr_def EsTy_def vimage_def)
     next
       apply_end(rule conjI) 
-      show "dom (tgtm (toSGr SG_ASD_3WTs)) = EsTy (toSGr SG_ASD_3WTs) {Some erelbi, Some ereluni, Some ecompbi, Some ecompuni}"
-        by (rule equalityI, rule subsetI, 
-          auto simp add: SG_ASD_3WTs_def toSGr_def EsTy_def vimage_def)
+      show "dom (tgtm (toSGr SG_ASD_3WTs_loop)) 
+        = EsTy (toSGr SG_ASD_3WTs_loop) {Some erelbi, Some ereluni, Some ecompbi, Some ecompuni}"
+        by (rule equalityI, 
+          auto simp add: SG_ASD_3WTs_loop_def toSGr_def EsTy_def vimage_def)
     next
       apply_end(rule conjI)
-      show "EsR (toSGr SG_ASD_3WTs) \<subseteq> EsId (toSGr SG_ASD_3WTs)"
-        by (simp add: EsR_def toSGr_def EsTy_def vimage_def SG_ASD_3WTs_def)
+      show "EsR (toSGr SG_ASD_3WTs_loop) \<subseteq> EsId (toSGr SG_ASD_3WTs_loop)"
+        by (simp add: EsR_def toSGr_def EsTy_def vimage_def SG_ASD_3WTs_loop_def)
     next
       apply_end(rule conjI)
-      show "srcm (toSGr SG_ASD_3WTs) ` EsTy (toSGr SG_ASD_3WTs) {Some ecompbi}
+      show "srcm (toSGr SG_ASD_3WTs_loop) ` EsTy (toSGr SG_ASD_3WTs_loop) {Some ecompbi}
         \<subseteq> {Some (rm 0 (val (Suc 0))), Some (sm (val (Suc 0)))}"
-        by (simp add: toSGr_def image_def SG_ASD_3WTs_def EsTy_def)
+        by (simp add: toSGr_def image_def SG_ASD_3WTs_loop_def EsTy_def)
     next
-      show "acyclicGr (inhG (toSGr SG_ASD_3WTs))"
+      show "acyclicGr (inhG (toSGr SG_ASD_3WTs_loop))"
         using h_wf_g by (simp add: inh_eq acyclicGr_def rtrancl_in inh_eq_consInh)(eval)
     qed
   qed
 
 (*'F_CD' Fragment*)
-definition F_ASD_3WTs :: "Fr_ls"
+definition F_ASD_3WTs_loop :: "Fr_ls"
 where
-   "F_ASD_3WTs \<equiv> \<lparr>sg_ls = SG_ASD_3WTs, 
+   "F_ASD_3WTs_loop \<equiv> \<lparr>sg_ls = SG_ASD_3WTs_loop, 
     tr_ls = []\<rparr>"
 
-value "consRefs F_ASD_3WTs"
+value "consRefs F_ASD_3WTs_loop"
 
 (* Well-formedness proof obligation of fragments"*)
-lemma wf_F_ASD_3WTs: "is_wf_fr (toFr F_ASD_3WTs)"
+lemma wf_F_ASD_3WTs_loop: "is_wf_fr (toFr F_ASD_3WTs_loop)"
   proof -
-    let ?refs_F_ASD_3WTs = "{}"
-    have h_ftotal_tr: "ftotal_on (tr (toFr F_ASD_3WTs)) (EsRP (sg (toFr F_ASD_3WTs))) V_A"
+    let ?refs_F_ASD_3WTs_loop = "{}"
+    have h_ftotal_tr: "ftotal_on (tr (toFr F_ASD_3WTs_loop)) (EsRP (sg (toFr F_ASD_3WTs_loop))) V_A"
       proof (simp add: ftotal_on_def)
         apply_end(rule conjI)
-        show "dom (tr (toFr F_ASD_3WTs)) = EsRP (sg (toFr F_ASD_3WTs))"
+        show "dom (tr (toFr F_ASD_3WTs_loop)) = EsRP (sg (toFr F_ASD_3WTs_loop))"
         proof
-          show "dom (tr (toFr F_ASD_3WTs)) \<subseteq> EsRP (sg (toFr F_ASD_3WTs))"
-            by (simp add: F_ASD_3WTs_def SG_ASD_3WTs_def toSGr_def toFr_def  
+          show "dom (tr (toFr F_ASD_3WTs_loop)) \<subseteq> EsRP (sg (toFr F_ASD_3WTs_loop))"
+            by (simp add: F_ASD_3WTs_loop_def SG_ASD_3WTs_loop_def toSGr_def toFr_def  
           SG_F_Props_def EsRP_def EsR_def NsP_def EsTy_def NsTy_def) 
         next
-          show "EsRP (sg (toFr F_ASD_3WTs)) \<subseteq> dom (tr (toFr F_ASD_3WTs))"
-            by (auto simp add: F_ASD_3WTs_def SG_ASD_3WTs_def toSGr_def toFr_def SG_F_Common_def 
+          show "EsRP (sg (toFr F_ASD_3WTs_loop)) \<subseteq> dom (tr (toFr F_ASD_3WTs_loop))"
+            by (auto simp add: F_ASD_3WTs_loop_def SG_ASD_3WTs_loop_def toSGr_def toFr_def SG_F_Common_def 
               SG_F_Props_def EsRP_def EsR_def NsP_def EsTy_def NsTy_def)
         qed
       next
-        show "ran (tr (toFr F_ASD_3WTs)) \<subseteq> V_A"
+        show "ran (tr (toFr F_ASD_3WTs_loop)) \<subseteq> V_A"
         using Ns_SG_F_ASD Ns_SG_F_Comps Ns_SG_F_Blocks Ns_SG_F_Common Ns_SG_F_VTypes
-        by (simp add: F_ASD_3WTs_def SG_ASD_3WTs_def toSGr_def toFr_def SG_F_Comps_def 
+        by (simp add: F_ASD_3WTs_loop_def SG_ASD_3WTs_loop_def toSGr_def toFr_def SG_F_Comps_def 
           SG_F_Blocks_def F_Common_def SG_F_Common_def F_VTypes_def SG_F_VTypes_def)
       qed
-      from wf_SG_ASD_3WTs have hb: "is_wf_sg (sg (toFr F_ASD_3WTs))"
-      by (simp add: toFr_def F_ASD_3WTs_def)
-    have refs_F_ASD_3WTs: "refs (toFr F_ASD_3WTs) = ?refs_F_ASD_3WTs"
+      from wf_SG_ASD_3WTs_loop have hb: "is_wf_sg (sg (toFr F_ASD_3WTs_loop))"
+      by (simp add: toFr_def F_ASD_3WTs_loop_def)
+    have refs_F_ASD_3WTs_loop: "refs (toFr F_ASD_3WTs_loop) = ?refs_F_ASD_3WTs_loop"
       using h_ftotal_tr hb by (simp add: refs_eq_consRefs, eval)
     show ?thesis
     proof (simp add: is_wf_fr_def)
       apply_end(rule conjI)
-      show "is_wf_sg (sg (toFr F_ASD_3WTs))"  
-        by (simp add: wf_SG_ASD_3WTs toFr_def F_ASD_3WTs_def)
+      show "is_wf_sg (sg (toFr F_ASD_3WTs_loop))"  
+        by (simp add: wf_SG_ASD_3WTs_loop toFr_def F_ASD_3WTs_loop_def)
     next
       apply_end(rule conjI) 
-      show "ftotal_on (tr (toFr F_ASD_3WTs)) (EsRP (sg (toFr F_ASD_3WTs))) V_A"
+      show "ftotal_on (tr (toFr F_ASD_3WTs_loop)) (EsRP (sg (toFr F_ASD_3WTs_loop))) V_A"
         by (simp add: h_ftotal_tr)
     next
       apply_end(rule conjI)  
-      show "inj_on (src (sg (toFr F_ASD_3WTs))) (EsRP (sg (toFr F_ASD_3WTs)))"
-        by (simp add: F_ASD_3WTs_def inj_on_def EsRP_def EsR_def NsP_def EsTy_def NsTy_def 
-          SG_ASD_3WTs_def toFr_def toSGr_def) 
+      show "inj_on (src (sg (toFr F_ASD_3WTs_loop))) (EsRP (sg (toFr F_ASD_3WTs_loop)))"
+        by (simp add: F_ASD_3WTs_loop_def inj_on_def EsRP_def EsR_def NsP_def EsTy_def NsTy_def 
+          SG_ASD_3WTs_loop_def toFr_def toSGr_def) 
     next
       apply_end(rule conjI)  
-      show "ran (src (sg (toFr F_ASD_3WTs)) |` EsRP (sg (toFr F_ASD_3WTs))) = NsP (sg (toFr F_ASD_3WTs))"
-        by (simp add: F_ASD_3WTs_def restrict_map_def NsP_def NsTy_def EsRP_def 
-          toFr_def SG_ASD_3WTs_def EsR_def EsTy_def toSGr_def vimage_def)
+      show "ran (src (sg (toFr F_ASD_3WTs_loop)) |` EsRP (sg (toFr F_ASD_3WTs_loop))) = NsP (sg (toFr F_ASD_3WTs_loop))"
+        by (simp add: F_ASD_3WTs_loop_def restrict_map_def NsP_def NsTy_def EsRP_def 
+          toFr_def SG_ASD_3WTs_loop_def EsR_def EsTy_def toSGr_def vimage_def)
     next
       apply_end(rule conjI)
-      show "\<forall>v. v \<in> NsP (sg (toFr F_ASD_3WTs)) \<longrightarrow> nonPRefsOf (toFr F_ASD_3WTs) v \<noteq> {}"
-        by (simp add: NsP_def NsTy_def nonPRefsOf_def refsOf_def refs_F_ASD_3WTs)
-          (simp add: F_ASD_3WTs_def SG_ASD_3WTs_def toFr_def toSGr_def)
+      show "\<forall>v. v \<in> NsP (sg (toFr F_ASD_3WTs_loop)) \<longrightarrow> nonPRefsOf (toFr F_ASD_3WTs_loop) v \<noteq> {}"
+        by (simp add: NsP_def NsTy_def nonPRefsOf_def refsOf_def refs_F_ASD_3WTs_loop)
+          (simp add: F_ASD_3WTs_loop_def SG_ASD_3WTs_loop_def toFr_def toSGr_def)
     next
       apply_end(rule conjI)
-      have h_wf_g: "is_wf_g (toSGr SG_ASD_3WTs)"
-        using Ns_SG_ASD_3WTs Es_SG_ASD_3WTs
-        by (simp add: is_wf_g_def SG_ASD_3WTs_def ftotal_on_def toSGr_def)
-      show "acyclic_fr (toFr F_ASD_3WTs)"
-        using  h_wf_g by (simp add: acyclic_fr_def refs_F_ASD_3WTs)
-          (simp add: inh_eq rtrancl_in inh_eq_consInh F_ASD_3WTs_def toFr_def, eval)
+      have h_wf_g: "is_wf_g (toSGr SG_ASD_3WTs_loop)"
+        using Ns_SG_ASD_3WTs_loop Es_SG_ASD_3WTs_loop
+        by (simp add: is_wf_g_def SG_ASD_3WTs_loop_def ftotal_on_def toSGr_def)
+      show "acyclic_fr (toFr F_ASD_3WTs_loop)"
+        using  h_wf_g by (simp add: acyclic_fr_def refs_F_ASD_3WTs_loop)
+          (simp add: inh_eq rtrancl_in inh_eq_consInh F_ASD_3WTs_loop_def toFr_def, eval)
     next
-      show "proxies_dont_inherit (toFr F_ASD_3WTs)"
+      show "proxies_dont_inherit (toFr F_ASD_3WTs_loop)"
         by (simp add: proxies_dont_inherit_def restrict_map_def NsP_def NsTy_def
-          F_ASD_3WTs_def toFr_def vimage_def SG_ASD_3WTs_def toSGr_def)
+          F_ASD_3WTs_loop_def toFr_def vimage_def SG_ASD_3WTs_loop_def toSGr_def)
     qed
   qed
 
 (*Define a model*. Update this later to conver connections*)
-definition SG_CD_3WTs :: "SGr_ls"
+definition SG_CD_3WTs_loop :: "SGr_ls"
 where
-  "SG_CD_3WTs = \<lparr>
+  "SG_CD_3WTs_loop = \<lparr>
     NsG=[''PrWaterTank'', ''PrValve'', ''PrTanksControl1'', 
       ''PrTanksControl2'', ''PrController'', ''CD_3WTs'', ''WTSys'',
       ''V'', ''WT1'', ''WT2'', ''WT3'', ''C'',
       ''TC1'', ''TC2'', ''v1'', ''v2'', ''w'', ''win1'', ''wout1'', ''win2'', 
-      ''wout2'', ''win3'', ''wout3'', ''C_w_win1'', ''C_wout1_win2'', ''C_wout2_win3'',
-      ''C_v1_v2'', ''PrValve_v2'', ''PrValve_w'', ''PrWaterTank_win'', 
-      ''PrWaterTank_wout'', ''PrController_v1''], 
+      ''wout2'', ''win3'', ''wout3'', ''win'', ''C_w_win1'', ''C_wout1_win2'', 
+      ''C_wout2_win3'', ''C_v1_v2'', ''C_wout3_win'',
+      ''PrValve_v2'', ''PrValve_w'', ''PrWaterTank_win'', 
+      ''PrWaterTank_wout'', ''PrController_v1'', ''PrController_win''], 
     EsG = [''ECD_WTSys'', ''ECD_V'', ''ECD_WT1'', ''ECD_WT2'', ''ECD_WT3'',   
       ''ECD_C'', ''ECD_TC1'', ''ECD_TC2'', ''ECD_C_v1_v2'', ''ECD_C_w_win1'', 
       ''ECD_C_wout1_win2'', ''ECD_C_wout2_win3'', 
-      ''E_C_v1'', ''E_V_v2'', ''E_V_w'',  ''E_WT1_win1'', ''E_WT1_wout1'', 
+      ''E_C_v1'', ''E_C_win'', ''E_V_v2'', ''E_V_w'',  ''E_WT1_win1'', ''E_WT1_wout1'', 
       ''E_WT2_win2'', ''E_WT2_wout2'', ''E_WT3_win3'', ''E_WT3_wout3'',
       ''E_C_v1_v2_src'', ''E_C_v1_v2_tgt'', ''E_C_w_win1_src'', ''E_C_w_win1_tgt'', 
       ''E_C_wout1_win2_src'', ''E_C_wout1_win2_tgt'', 
       ''E_C_wout2_win3_src'', ''E_C_wout2_win3_tgt'', 
+      ''E_C_wout3_win_src'', ''E_C_wout3_win_tgt'',
       ''ETC1_V'', ''ETC1_WT1'', ''ETC2_WT2'',
       ''ETC2_WT3'', ''EWTSys_TC1'', ''EWTSys_TC2'', ''EWTSys_C'', 
-      ''E_v1_ty'', ''E_v2_ty'', ''E_w_ty'', ''E_win1_ty'', ''E_wout1_ty'',
-      ''E_win2_ty'', ''E_wout2_ty'', ''E_win3_ty'', ''E_wout3_ty'',
+      ''E_v1_ty'', ''E_win_ty'', ''E_v2_ty'', ''E_w_ty'', ''E_win1_ty'', 
+      ''E_wout1_ty'', ''E_win2_ty'', ''E_wout2_ty'', ''E_win3_ty'', ''E_wout3_ty'',
       ''ERPrWaterTank'', ''ERPrValve'', ''ERPrTanksControl1'', ''ERPrTanksControl2'', 
       ''ERPrController'', ''ERPrValve_v2'', ''ERPrValve_w'', ''ERPrWaterTank_win'',
-      ''ERPrWaterTank_wout'', ''ERPrController_v1''], 
+      ''ERPrWaterTank_wout'', ''ERPrController_v1'', ''ERPrController_win''], 
     srcG =  [
       (''ECD_WTSys'', ''CD_3WTs''), (''ECD_V'', ''CD_3WTs''), 
       (''ECD_WT1'', ''CD_3WTs''), (''ECD_WT2'', ''CD_3WTs''),
@@ -314,7 +320,7 @@ where
       (''ECD_TC1'', ''CD_3WTs''), (''ECD_TC2'', ''CD_3WTs''),
       (''ECD_C_v1_v2'', ''CD_3WTs''), (''ECD_C_w_win1'', ''CD_3WTs''),
       (''ECD_C_wout1_win2'', ''CD_3WTs''), (''ECD_C_wout2_win3'', ''CD_3WTs''),
-      (''E_C_v1'', ''C''),
+      (''E_C_v1'', ''C''), (''E_C_win'', ''C''),
       (''E_V_v2'', ''V''), (''E_V_w'', ''V''),  
       (''E_WT1_win1'', ''WT1''), (''E_WT1_wout1'', ''WT1''), 
       (''E_WT2_win2'', ''WT2''), (''E_WT2_wout2'', ''WT2''), 
@@ -323,11 +329,12 @@ where
       (''E_C_w_win1_src'', ''C_w_win1''), (''E_C_w_win1_tgt'', ''C_w_win1''),
       (''E_C_wout1_win2_src'', ''C_wout1_win2''), (''E_C_wout1_win2_tgt'', ''C_wout1_win2''), 
       (''E_C_wout2_win3_src'', ''C_wout2_win3''), (''E_C_wout2_win3_tgt'', ''C_wout2_win3''),
+      (''E_C_wout3_win_src'', ''C_wout3_win''), (''E_C_wout3_win_tgt'', ''C_wout3_win''),
       (''ETC1_V'', ''TC1''),
       (''ETC1_WT1'', ''TC1''), (''ETC2_WT2'', ''TC2''),
       (''ETC2_WT3'', ''TC2''), (''EWTSys_TC1'', ''WTSys''), 
       (''EWTSys_TC2'', ''WTSys''), (''EWTSys_C'', ''WTSys''),
-      (''E_v1_ty'', ''v1''), (''E_v2_ty'', ''v2''), 
+      (''E_v1_ty'', ''v1''), (''E_win_ty'', ''win''), (''E_v2_ty'', ''v2''), 
       (''E_w_ty'', ''w''), (''E_win1_ty'', ''win1''), 
       (''E_wout1_ty'', ''wout1''),
       (''E_win2_ty'', ''win2''), (''E_wout2_ty'', ''wout2''), 
@@ -339,7 +346,8 @@ where
       (''ERPrValve_v2'', ''PrValve_v2''), (''ERPrValve_w'', ''PrValve_w''), 
       (''ERPrWaterTank_win'', ''PrWaterTank_win''),
       (''ERPrWaterTank_wout'', ''PrWaterTank_wout''), 
-      (''ERPrController_v1'', ''PrController_v1'')], 
+      (''ERPrController_v1'', ''PrController_v1''), 
+      (''ERPrController_win'', ''PrController_win'')], 
     tgtG =  [
       (''ECD_WTSys'', ''WTSys''), (''ECD_V'', ''V''), 
       (''ECD_WT1'', ''WT1''), (''ECD_WT2'', ''WT2''),
@@ -348,7 +356,7 @@ where
       (''ECD_C_v1_v2'', ''C_v1_v2''), (''ECD_C_w_win1'', ''C_w_win1''),
       (''ECD_C_wout1_win2'', ''C_wout1_win2''), 
       (''ECD_C_wout2_win3'', ''C_wout2_win3''),
-      (''E_C_v1'', ''v1''),
+      (''E_C_v1'', ''v1''), (''E_C_win'', ''win''),
       (''E_V_v2'', ''v2''), (''E_V_w'', ''w''),  
       (''E_WT1_win1'', ''win1''), (''E_WT1_wout1'', ''wout1''), 
       (''E_WT2_win2'', ''win2''), (''E_WT2_wout2'', ''wout2''), 
@@ -357,11 +365,13 @@ where
       (''E_C_w_win1_src'', ''w''), (''E_C_w_win1_tgt'', ''win1''),
       (''E_C_wout1_win2_src'', ''wout1''), (''E_C_wout1_win2_tgt'', ''win2''), 
       (''E_C_wout2_win3_src'', ''wout2''), (''E_C_wout2_win3_tgt'', ''win3''),
+      (''E_C_wout3_win_src'', ''wout3''), (''E_C_wout3_win_tgt'', ''win''),
       (''ETC1_V'', ''V''),
       (''ETC1_WT1'', ''WT1''), (''ETC2_WT2'', ''WT2''),
       (''ETC2_WT3'', ''WT3''), (''EWTSys_TC1'', ''TC1''), 
       (''EWTSys_TC2'', ''TC2''), (''EWTSys_C'', ''C''),
-      (''E_v1_ty'', ''PrController_v1''), (''E_v2_ty'', ''PrValve_v2''), 
+      (''E_v1_ty'', ''PrController_v1''), (''E_win_ty'', ''PrController_win''), 
+      (''E_v2_ty'', ''PrValve_v2''), 
       (''E_w_ty'', ''PrValve_w''), (''E_win1_ty'', ''PrWaterTank_win''), 
       (''E_wout1_ty'', ''PrWaterTank_wout''),
       (''E_win2_ty'', ''PrWaterTank_win''), (''E_wout2_ty'', ''PrWaterTank_wout''), 
@@ -373,7 +383,8 @@ where
       (''ERPrValve_v2'', ''PrValve_v2''), (''ERPrValve_w'', ''PrValve_w''), 
       (''ERPrWaterTank_win'', ''PrWaterTank_win''),
       (''ERPrWaterTank_wout'', ''PrWaterTank_wout''), 
-      (''ERPrController_v1'', ''PrController_v1'')],
+      (''ERPrController_v1'', ''PrController_v1''),
+      (''ERPrController_win'', ''PrController_win'')],
    ntyG =[(''PrWaterTank'',  nprxy), (''PrValve'', nprxy), 
         (''PrTanksControl1'', nprxy), (''PrTanksControl2'', nprxy),
         (''PrController'', nprxy), (''CD_3WTs'',  nnrml),
@@ -382,12 +393,14 @@ where
         (''C'', nnrml), (''TC1'', nnrml), (''TC2'', nnrml), 
         (''v1'', nnrml), (''v2'', nnrml), (''w'', nnrml), (''win1'', nnrml),
         (''wout1'', nnrml), (''win2'', nnrml), (''wout2'', nnrml), 
-        (''win3'', nnrml), (''wout3'', nnrml),
+        (''win3'', nnrml), (''wout3'', nnrml), (''win'', nnrml),
         (''C_w_win1'', nnrml), (''C_wout1_win2'', nnrml), 
         (''C_wout2_win3'', nnrml), (''C_v1_v2'', nnrml), 
+        (''C_wout3_win'', nnrml), 
         (''PrValve_v2'', nprxy), (''PrValve_w'', nprxy), 
         (''PrWaterTank_win'', nprxy),
-        (''PrWaterTank_wout'', nprxy), (''PrController_v1'', nprxy)],
+        (''PrWaterTank_wout'', nprxy), (''PrController_v1'', nprxy), 
+        (''PrController_win'', nprxy)],
       etyG =[
         (''ECD_WTSys'', elnk), (''ECD_V'', elnk), 
         (''ECD_WT1'', elnk), (''ECD_WT2'', elnk),
@@ -396,7 +409,7 @@ where
         (''ECD_C_v1_v2'', elnk), (''ECD_C_w_win1'', elnk),
         (''ECD_C_wout1_win2'', elnk), 
         (''ECD_C_wout2_win3'', elnk),
-        (''E_C_v1'', elnk),
+        (''E_C_v1'', elnk), (''E_C_win'', elnk),
         (''E_V_v2'', elnk), (''E_V_w'', elnk),  
         (''E_WT1_win1'', elnk), (''E_WT1_wout1'', elnk), 
         (''E_WT2_win2'', elnk), (''E_WT2_wout2'', elnk), 
@@ -405,12 +418,15 @@ where
         (''E_C_w_win1_src'', elnk), (''E_C_w_win1_tgt'', elnk),
         (''E_C_wout1_win2_src'', elnk), (''E_C_wout1_win2_tgt'', elnk), 
         (''E_C_wout2_win3_src'', elnk), (''E_C_wout2_win3_tgt'', elnk),
+        (''E_C_wout3_win_src'', elnk), 
+        (''E_C_wout3_win_tgt'', elnk),
         (''ETC1_V'', elnk),
         (''ETC1_WT1'', elnk), (''ETC2_WT2'', elnk),
         (''ETC2_WT3'', elnk), (''EWTSys_TC1'', elnk), 
         (''EWTSys_TC2'', elnk), 
         (''EWTSys_C'', elnk), 
-        (''E_v1_ty'', elnk), (''E_v2_ty'', elnk), 
+        (''E_v1_ty'', elnk), (''E_win_ty'', elnk),
+        (''E_v2_ty'', elnk), 
         (''E_w_ty'', elnk), (''E_win1_ty'', elnk), 
         (''E_wout1_ty'', elnk),
         (''E_win2_ty'', elnk), (''E_wout2_ty'', elnk), 
@@ -422,234 +438,247 @@ where
         (''ERPrValve_v2'', eref), (''ERPrValve_w'', eref), 
         (''ERPrWaterTank_win'', eref),
         (''ERPrWaterTank_wout'', eref), 
-        (''ERPrController_v1'', eref)],
+        (''ERPrController_v1'', eref), 
+        (''ERPrController_win'', eref)],
       srcmG = [], 
       tgtmG = []\<rparr>"
 
 axiomatization
 where
-  Es_SG_CD_3WTs: "Es (toSGr SG_CD_3WTs) \<subseteq> E_A"
-  and Ns_SG_CD_3WTs: "Ns (toSGr SG_CD_3WTs) \<subseteq> V_A"
+  Es_SG_CD_3WTs_loop: "Es (toSGr SG_CD_3WTs_loop) \<subseteq> E_A"
+  and Ns_SG_CD_3WTs_loop: "Ns (toSGr SG_CD_3WTs_loop) \<subseteq> V_A"
 
-value "consInh SG_CD_3WTs"
+value "consInh SG_CD_3WTs_loop"
 
-lemma wf_SG_CD_3WTs: "is_wf_sg (toSGr SG_CD_3WTs)"
+lemma wf_SG_CD_3WTs_loop: "is_wf_sg (toSGr SG_CD_3WTs_loop)"
   proof -
-    have h_wf_g: "is_wf_g (toSGr SG_CD_3WTs)"
+    have h_wf_g: "is_wf_g (toSGr SG_CD_3WTs_loop)"
     proof (simp add: is_wf_g_def, rule conjI)
-      show "Ns (toSGr SG_CD_3WTs) \<subseteq> V_A"
-      using Ns_SG_CD_3WTs by (simp add: SG_CD_3WTs_def)
+      show "Ns (toSGr SG_CD_3WTs_loop) \<subseteq> V_A"
+      using Ns_SG_CD_3WTs_loop by (simp add: SG_CD_3WTs_loop_def)
     next
       apply_end(rule conjI)
-      show "Es (toSGr SG_CD_3WTs) \<subseteq> E_A"
-      using Es_SG_CD_3WTs by (simp add: SG_CD_3WTs_def)
+      show "Es (toSGr SG_CD_3WTs_loop) \<subseteq> E_A"
+      using Es_SG_CD_3WTs_loop by (simp add: SG_CD_3WTs_loop_def)
     next
       apply_end(rule conjI)
-      show "ftotal_on (src (toSGr SG_CD_3WTs)) (Es (toSGr SG_CD_3WTs)) (Ns (toSGr SG_CD_3WTs))"
-      by (simp add: SG_CD_3WTs_def ftotal_on_def toSGr_def)
+      show "ftotal_on (src (toSGr SG_CD_3WTs_loop)) (Es (toSGr SG_CD_3WTs_loop)) (Ns (toSGr SG_CD_3WTs_loop))"
+      by (simp add: SG_CD_3WTs_loop_def ftotal_on_def toSGr_def)
     next
-      show "ftotal_on (tgt (toSGr SG_CD_3WTs)) (Es (toSGr SG_CD_3WTs)) (Ns (toSGr SG_CD_3WTs))"
-      by (simp add: SG_CD_3WTs_def ftotal_on_def toSGr_def)
+      show "ftotal_on (tgt (toSGr SG_CD_3WTs_loop)) (Es (toSGr SG_CD_3WTs_loop)) (Ns (toSGr SG_CD_3WTs_loop))"
+      by (simp add: SG_CD_3WTs_loop_def ftotal_on_def toSGr_def)
     qed      
     show ?thesis
     proof (simp add: is_wf_sg_def, rule conjI)
-      show "is_wf_g (toSGr SG_CD_3WTs)"
+      show "is_wf_g (toSGr SG_CD_3WTs_loop)"
         using h_wf_g by simp
     next
       apply_end(rule conjI)
-      show "ftotal_on (nty (toSGr SG_CD_3WTs)) (Ns (toSGr SG_CD_3WTs)) SGNTy_set"
-        by (simp add: ftotal_on_def SGNTy_set_def SG_CD_3WTs_def toSGr_def)
+      show "ftotal_on (nty (toSGr SG_CD_3WTs_loop)) (Ns (toSGr SG_CD_3WTs_loop)) SGNTy_set"
+        by (simp add: ftotal_on_def SGNTy_set_def SG_CD_3WTs_loop_def toSGr_def)
     next
       apply_end(rule conjI) 
-      show "ftotal_on (ety (toSGr SG_CD_3WTs)) (Es (toSGr SG_CD_3WTs)) SGETy_set"
+      show "ftotal_on (ety (toSGr SG_CD_3WTs_loop)) (Es (toSGr SG_CD_3WTs_loop)) SGETy_set"
         by (simp add: ftotal_on_def, rule conjI, rule equalityI)
-        (simp_all add: SGNTy_set_def SG_CD_3WTs_def toSGr_def SGETy_set_def)
+        (simp_all add: SGNTy_set_def SG_CD_3WTs_loop_def toSGr_def SGETy_set_def)
     next
       apply_end(rule conjI) 
-      show "dom (srcm (toSGr SG_CD_3WTs)) = EsTy (toSGr SG_CD_3WTs) {Some erelbi, Some ecompbi}"
-        by (simp add: SG_CD_3WTs_def toSGr_def EsTy_def vimage_def)
+      show "dom (srcm (toSGr SG_CD_3WTs_loop)) = EsTy (toSGr SG_CD_3WTs_loop) {Some erelbi, Some ecompbi}"
+        by (simp add: SG_CD_3WTs_loop_def toSGr_def EsTy_def vimage_def)
     next
       apply_end(rule conjI) 
-      show "dom (tgtm (toSGr SG_CD_3WTs)) = EsTy (toSGr SG_CD_3WTs) {Some erelbi, Some ereluni, Some ecompbi, Some ecompuni}"
-        by (auto simp add: SG_CD_3WTs_def toSGr_def EsTy_def vimage_def)
+      show "dom (tgtm (toSGr SG_CD_3WTs_loop)) = EsTy (toSGr SG_CD_3WTs_loop) {Some erelbi, Some ereluni, Some ecompbi, Some ecompuni}"
+        by (auto simp add: SG_CD_3WTs_loop_def toSGr_def EsTy_def vimage_def)
     next
       apply_end(rule conjI)
-      show "EsR (toSGr SG_CD_3WTs) \<subseteq> EsId (toSGr SG_CD_3WTs)"
+      show "EsR (toSGr SG_CD_3WTs_loop) \<subseteq> EsId (toSGr SG_CD_3WTs_loop)"
       proof
         fix x
-        assume " x \<in> EsR (toSGr SG_CD_3WTs)"
-        then show "x \<in> EsId (toSGr SG_CD_3WTs)"
-        by (auto simp add: EsR_def toSGr_def EsTy_def vimage_def SG_CD_3WTs_def EsId_def
+        assume " x \<in> EsR (toSGr SG_CD_3WTs_loop)"
+        then show "x \<in> EsId (toSGr SG_CD_3WTs_loop)"
+        by (auto simp add: EsR_def toSGr_def EsTy_def vimage_def SG_CD_3WTs_loop_def EsId_def
           split: if_splits)
       qed
     next
       apply_end(rule conjI)
-      show "srcm (toSGr SG_CD_3WTs) ` EsTy (toSGr SG_CD_3WTs) {Some ecompbi}
+      show "srcm (toSGr SG_CD_3WTs_loop) ` EsTy (toSGr SG_CD_3WTs_loop) {Some ecompbi}
         \<subseteq> {Some (rm 0 (val (Suc 0))), Some (sm (val (Suc 0)))}"
-        by (simp add: toSGr_def image_def SG_CD_3WTs_def EsTy_def)
+        by (simp add: toSGr_def image_def SG_CD_3WTs_loop_def EsTy_def)
     next
-      show "acyclicGr (inhG (toSGr SG_CD_3WTs))"
+      show "acyclicGr (inhG (toSGr SG_CD_3WTs_loop))"
         using h_wf_g by (simp add: inh_eq acyclicGr_def rtrancl_in inh_eq_consInh)(eval)
     qed
   qed
 
 (*'F_CD' Fragment*)
-definition F_CD_3WTs :: "Fr_ls"
+definition F_CD_3WTs_loop :: "Fr_ls"
 where
-   "F_CD_3WTs \<equiv> \<lparr>sg_ls = SG_CD_3WTs, 
+   "F_CD_3WTs_loop \<equiv> \<lparr>sg_ls = SG_CD_3WTs_loop, 
     tr_ls = [(''ERPrWaterTank'', ''WaterTank''), (''ERPrValve'', ''Valve''), 
     (''ERPrTanksControl1'', ''TanksControl1''), (''ERPrTanksControl2'', ''TanksControl2''),
     (''ERPrController'', ''Controller''),
     (''ERPrValve_v2'', ''Valve_v2''), (''ERPrValve_w'', ''Valve_w''), 
     (''ERPrWaterTank_win'', ''WaterTank_win''),
     (''ERPrWaterTank_wout'', ''WaterTank_wout''), 
-    (''ERPrController_v1'', ''Controller_v1'')]\<rparr>"
+    (''ERPrController_v1'', ''Controller_v1''),
+    (''ERPrController_win'', ''Controller_win'')]\<rparr>"
 
-value "consRefs F_CD_3WTs"
+value "consRefs F_CD_3WTs_loop"
 
-value "consUFs [F_ASD_3WTs, F_CD_3WTs]"
+value "consUFs [F_ASD_3WTs_loop, F_CD_3WTs_loop]"
 
 (* Well-formedness proof obligation of fragments"*)
-lemma wf_F_CD_3WTs: "is_wf_fr (toFr F_CD_3WTs)"
+lemma wf_F_CD_3WTs_loop: "is_wf_fr (toFr F_CD_3WTs_loop)"
   proof -
-    let ?refs_F_CD_3WTs = "{(''PrWaterTank'', ''WaterTank''), 
+    let ?refs_F_CD_3WTs_loop = "{(''PrWaterTank'', ''WaterTank''), 
       (''PrValve'', ''Valve''),
       (''PrTanksControl1'', ''TanksControl1''), 
       (''PrTanksControl2'', ''TanksControl2''),
-      (''PrController'', ''Controller''), 
+      (''PrController'', ''Controller''),   
       (''PrValve_v2'', ''Valve_v2''),
       (''PrValve_w'', ''Valve_w''), 
       (''PrWaterTank_win'', ''WaterTank_win''),
       (''PrWaterTank_wout'', ''WaterTank_wout''), 
-      (''PrController_v1'', ''Controller_v1'')}"
-    have h_EsRP: "EsRP (sg (toFr F_CD_3WTs)) = {''ERPrWaterTank'', ''ERPrValve'',
+      (''PrController_v1'', ''Controller_v1''),
+      (''PrController_win'', ''Controller_win'')}"
+    have h_EsRP: "EsRP (sg (toFr F_CD_3WTs_loop)) = {''ERPrWaterTank'', ''ERPrValve'',
           ''ERPrTanksControl1'', ''ERPrTanksControl2'',
           ''ERPrController'', ''ERPrValve_v2'',
           ''ERPrValve_w'', ''ERPrWaterTank_win'', 
-          ''ERPrWaterTank_wout'', ''ERPrController_v1''}"
+          ''ERPrWaterTank_wout'', ''ERPrController_v1'', ''ERPrController_win''}"
       by (rule equalityI, rule subsetI, simp_all add: EsRP_def EsR_def EsTy_def NsP_def NsTy_def 
-        toFr_def F_CD_3WTs_def toSGr_def SG_CD_3WTs_def split: if_splits)
-    have h_ftotal_tr: "ftotal_on (tr (toFr F_CD_3WTs)) (EsRP (sg (toFr F_CD_3WTs))) V_A"
-      using Ns_SG_ASD_3WTs
-      by (simp add: h_EsRP)(simp add: F_CD_3WTs_def SG_CD_3WTs_def toSGr_def toFr_def  
-          ftotal_on_def SG_ASD_3WTs_def) 
-    from wf_SG_CD_3WTs have hb: "is_wf_sg (sg (toFr F_CD_3WTs))"
-      by (simp add: toFr_def F_CD_3WTs_def)
-    have refs_F_CD_3WTs: "refs (toFr F_CD_3WTs) = ?refs_F_CD_3WTs"
+        toFr_def F_CD_3WTs_loop_def toSGr_def SG_CD_3WTs_loop_def split: if_splits)
+    have h_ftotal_tr: "ftotal_on (tr (toFr F_CD_3WTs_loop)) (EsRP (sg (toFr F_CD_3WTs_loop))) V_A"
+      using Ns_SG_ASD_3WTs_loop
+      by (simp add: h_EsRP)(simp add: F_CD_3WTs_loop_def SG_CD_3WTs_loop_def toSGr_def toFr_def  
+          ftotal_on_def SG_ASD_3WTs_loop_def) 
+    from wf_SG_CD_3WTs_loop have hb: "is_wf_sg (sg (toFr F_CD_3WTs_loop))"
+      by (simp add: toFr_def F_CD_3WTs_loop_def)
+    have refs_F_CD_3WTs_loop: "refs (toFr F_CD_3WTs_loop) = ?refs_F_CD_3WTs_loop"
       using h_ftotal_tr hb by (simp add: refs_eq_consRefs, eval)
-    have h_NsP: "NsP (sg (toFr F_CD_3WTs)) = {''PrWaterTank'', 
+    have h_NsP: "NsP (sg (toFr F_CD_3WTs_loop)) = {''PrWaterTank'', 
       ''PrValve'', ''PrTanksControl1'', ''PrTanksControl2'', 
       ''PrController'', ''PrValve_v2'', ''PrValve_w'', ''PrWaterTank_win'', 
-      ''PrWaterTank_wout'', ''PrController_v1''}"
-      by (rule equalityI, rule subsetI, simp_all add: F_CD_3WTs_def NsP_def NsTy_def 
-        toFr_def SG_CD_3WTs_def toSGr_def vimage_def split: if_splits)
+      ''PrWaterTank_wout'', ''PrController_v1'', ''PrController_win''}"
+      by (rule equalityI, rule subsetI, simp_all add: F_CD_3WTs_loop_def NsP_def NsTy_def 
+        toFr_def SG_CD_3WTs_loop_def toSGr_def vimage_def split: if_splits)
     show ?thesis
     proof (simp add: is_wf_fr_def)
       apply_end(rule conjI)
-      show "is_wf_sg (sg (toFr F_CD_3WTs))"  
-        by (simp add: wf_SG_CD_3WTs toFr_def F_CD_3WTs_def)
+      show "is_wf_sg (sg (toFr F_CD_3WTs_loop))"  
+        by (simp add: wf_SG_CD_3WTs_loop toFr_def F_CD_3WTs_loop_def)
     next
       apply_end(rule conjI) 
-      show "ftotal_on (tr (toFr F_CD_3WTs)) (EsRP (sg (toFr F_CD_3WTs))) V_A"
+      show "ftotal_on (tr (toFr F_CD_3WTs_loop)) (EsRP (sg (toFr F_CD_3WTs_loop))) V_A"
         by (simp add: h_ftotal_tr)
     next
       apply_end(rule conjI)  
-      show "inj_on (src (sg (toFr F_CD_3WTs))) (EsRP (sg (toFr F_CD_3WTs)))"
+      show "inj_on (src (sg (toFr F_CD_3WTs_loop))) (EsRP (sg (toFr F_CD_3WTs_loop)))"
       proof (simp add: inj_on_def, clarify)
         fix x y
-        assume "x \<in> EsRP (sg (toFr F_CD_3WTs))"
-          and "y \<in> EsRP (sg (toFr F_CD_3WTs))"
-          and "src (sg (toFr F_CD_3WTs)) x = src (sg (toFr F_CD_3WTs)) y"
+        assume "x \<in> EsRP (sg (toFr F_CD_3WTs_loop))"
+          and "y \<in> EsRP (sg (toFr F_CD_3WTs_loop))"
+          and "src (sg (toFr F_CD_3WTs_loop)) x = src (sg (toFr F_CD_3WTs_loop)) y"
         then show "x = y"
-        by (simp add: h_EsRP) (simp add: F_CD_3WTs_def  
-          SG_CD_3WTs_def toFr_def toSGr_def split: if_splits) 
+        by (simp add: h_EsRP) (simp add: F_CD_3WTs_loop_def  
+          SG_CD_3WTs_loop_def toFr_def toSGr_def split: if_splits) 
       qed
     next
       apply_end(rule conjI)  
-      show "ran (src (sg (toFr F_CD_3WTs)) |` EsRP (sg (toFr F_CD_3WTs))) = NsP (sg (toFr F_CD_3WTs))"
-      by (simp add: h_EsRP h_NsP)(rule equalityI, simp_all add: F_CD_3WTs_def SG_CD_3WTs_def  
+      show "ran (src (sg (toFr F_CD_3WTs_loop)) |` EsRP (sg (toFr F_CD_3WTs_loop))) = NsP (sg (toFr F_CD_3WTs_loop))"
+      by (simp add: h_EsRP h_NsP)(rule equalityI, simp_all add: F_CD_3WTs_loop_def SG_CD_3WTs_loop_def  
         toFr_def toSGr_def)
     next
       apply_end(rule conjI)
-      show "\<forall>v. v \<in> NsP (sg (toFr F_CD_3WTs)) \<longrightarrow> nonPRefsOf (toFr F_CD_3WTs) v \<noteq> {}"
+      show "\<forall>v. v \<in> NsP (sg (toFr F_CD_3WTs_loop)) \<longrightarrow> nonPRefsOf (toFr F_CD_3WTs_loop) v \<noteq> {}"
       proof (rule allI, rule impI)
         fix v
-        assume h1: "v \<in> NsP (sg (toFr F_CD_3WTs))"
-        then show "nonPRefsOf (toFr F_CD_3WTs) v \<noteq> {}"
+        assume h1: "v \<in> NsP (sg (toFr F_CD_3WTs_loop))"
+        then show "nonPRefsOf (toFr F_CD_3WTs_loop) v \<noteq> {}"
         proof (case_tac  "v = ''PrWaterTank''")
           assume "v = ''PrWaterTank''"
-          then show "nonPRefsOf (toFr F_CD_3WTs) v \<noteq> {}"
-            by (simp add: h_NsP nonPRefsOf_def refsOf_def refs_F_CD_3WTs trancl_in)
+          then show "nonPRefsOf (toFr F_CD_3WTs_loop) v \<noteq> {}"
+            by (simp add: h_NsP nonPRefsOf_def refsOf_def refs_F_CD_3WTs_loop trancl_in)
         next  
           assume h2: "v \<noteq> ''PrWaterTank''"
-          then show "nonPRefsOf (toFr F_CD_3WTs) v \<noteq> {}"
+          then show "nonPRefsOf (toFr F_CD_3WTs_loop) v \<noteq> {}"
           proof (case_tac  "v = ''PrValve''")
             assume "v = ''PrValve''"
-            then show "nonPRefsOf (toFr F_CD_3WTs) v \<noteq> {}"
-              by (simp add: h_NsP nonPRefsOf_def refsOf_def refs_F_CD_3WTs trancl_in)
+            then show "nonPRefsOf (toFr F_CD_3WTs_loop) v \<noteq> {}"
+              by (simp add: h_NsP nonPRefsOf_def refsOf_def refs_F_CD_3WTs_loop trancl_in)
           next
             assume h3: "v \<noteq> ''PrValve''"
-            then show "nonPRefsOf (toFr F_CD_3WTs) v \<noteq> {}"
+            then show "nonPRefsOf (toFr F_CD_3WTs_loop) v \<noteq> {}"
             proof (case_tac  "v = ''PrTanksControl1''")
               assume "v = ''PrTanksControl1''"
-              then show "nonPRefsOf (toFr F_CD_3WTs) v \<noteq> {}"
-                by (simp add: h_NsP nonPRefsOf_def refsOf_def refs_F_CD_3WTs trancl_in)
+              then show "nonPRefsOf (toFr F_CD_3WTs_loop) v \<noteq> {}"
+                by (simp add: h_NsP nonPRefsOf_def refsOf_def refs_F_CD_3WTs_loop trancl_in)
             next
               assume h4: "v \<noteq> ''PrTanksControl1''"
-              then show "nonPRefsOf (toFr F_CD_3WTs) v \<noteq> {}"
+              then show "nonPRefsOf (toFr F_CD_3WTs_loop) v \<noteq> {}"
               proof (case_tac  "v = ''PrTanksControl2''")
                 assume "v = ''PrTanksControl2''"
-                then show "nonPRefsOf (toFr F_CD_3WTs) v \<noteq> {}"
-                  by (simp add: h_NsP nonPRefsOf_def refsOf_def refs_F_CD_3WTs trancl_in)
+                then show "nonPRefsOf (toFr F_CD_3WTs_loop) v \<noteq> {}"
+                  by (simp add: h_NsP nonPRefsOf_def refsOf_def refs_F_CD_3WTs_loop trancl_in)
               next
                 assume h5: "v \<noteq> ''PrTanksControl2''"
-                then show "nonPRefsOf (toFr F_CD_3WTs) v \<noteq> {}"
+                then show "nonPRefsOf (toFr F_CD_3WTs_loop) v \<noteq> {}"
                 proof (case_tac  "v = ''PrController''")
                   assume "v = ''PrController''"
-                  then show "nonPRefsOf (toFr F_CD_3WTs) v \<noteq> {}"
-                    by (simp add: h_NsP nonPRefsOf_def refsOf_def refs_F_CD_3WTs trancl_in)
+                  then show "nonPRefsOf (toFr F_CD_3WTs_loop) v \<noteq> {}"
+                    by (simp add: h_NsP nonPRefsOf_def refsOf_def refs_F_CD_3WTs_loop trancl_in)
                 next
                   assume h6: "v \<noteq> ''PrController''"
-                  then show "nonPRefsOf (toFr F_CD_3WTs) v \<noteq> {}"
+                  then show "nonPRefsOf (toFr F_CD_3WTs_loop) v \<noteq> {}"
                   proof (case_tac "v = ''PrValve_v2''")
                     assume "v = ''PrValve_v2''"
-                    then show "nonPRefsOf (toFr F_CD_3WTs) v \<noteq> {}"
-                      by (simp add: h_NsP nonPRefsOf_def refsOf_def refs_F_CD_3WTs trancl_in)
+                    then show "nonPRefsOf (toFr F_CD_3WTs_loop) v \<noteq> {}"
+                      by (simp add: h_NsP nonPRefsOf_def refsOf_def refs_F_CD_3WTs_loop trancl_in)
                   next
                     assume h7: "v \<noteq> ''PrValve_v2''"
-                    then show "nonPRefsOf (toFr F_CD_3WTs) v \<noteq> {}"
+                    then show "nonPRefsOf (toFr F_CD_3WTs_loop) v \<noteq> {}"
                     proof (case_tac "v = ''PrValve_w''")
                       assume "v = ''PrValve_w''"
-                      then show "nonPRefsOf (toFr F_CD_3WTs) v \<noteq> {}"
-                        by (simp add: h_NsP nonPRefsOf_def refsOf_def refs_F_CD_3WTs trancl_in)
+                      then show "nonPRefsOf (toFr F_CD_3WTs_loop) v \<noteq> {}"
+                        by (simp add: h_NsP nonPRefsOf_def refsOf_def refs_F_CD_3WTs_loop trancl_in)
                     next
                       assume h8: "v \<noteq> ''PrValve_w''"
-                      then show "nonPRefsOf (toFr F_CD_3WTs) v \<noteq> {}"
+                      then show "nonPRefsOf (toFr F_CD_3WTs_loop) v \<noteq> {}"
                       proof (case_tac "v = ''PrWaterTank_win''")
                         assume "v = ''PrWaterTank_win''"
-                        then show "nonPRefsOf (toFr F_CD_3WTs) v \<noteq> {}"
-                          by (simp add: h_NsP nonPRefsOf_def refsOf_def refs_F_CD_3WTs trancl_in)
+                        then show "nonPRefsOf (toFr F_CD_3WTs_loop) v \<noteq> {}"
+                          by (simp add: h_NsP nonPRefsOf_def refsOf_def refs_F_CD_3WTs_loop trancl_in)
                       next
                         assume h9: "v \<noteq> ''PrWaterTank_win''"
-                        then show "nonPRefsOf (toFr F_CD_3WTs) v \<noteq> {}"
+                        then show "nonPRefsOf (toFr F_CD_3WTs_loop) v \<noteq> {}"
                         proof (case_tac "v = ''PrWaterTank_wout''")
                           assume "v = ''PrWaterTank_wout''"
-                          then show "nonPRefsOf (toFr F_CD_3WTs) v \<noteq> {}"
-                            by (simp add: h_NsP nonPRefsOf_def refsOf_def refs_F_CD_3WTs trancl_in)
+                          then show "nonPRefsOf (toFr F_CD_3WTs_loop) v \<noteq> {}"
+                            by (simp add: h_NsP nonPRefsOf_def refsOf_def refs_F_CD_3WTs_loop trancl_in)
                         next
                           assume h10: "v \<noteq> ''PrWaterTank_wout''"
-                          then show "nonPRefsOf (toFr F_CD_3WTs) v \<noteq> {}"
+                          then show "nonPRefsOf (toFr F_CD_3WTs_loop) v \<noteq> {}"
                           using h2 h3 h4 h5 h6 h7 h8 h9 
                           proof (case_tac "v = ''PrController_v1''")
                             assume "v = ''PrController_v1''"
-                            then show "nonPRefsOf (toFr F_CD_3WTs) v \<noteq> {}"
-                              by (simp add: h_NsP nonPRefsOf_def refsOf_def refs_F_CD_3WTs 
+                            then show "nonPRefsOf (toFr F_CD_3WTs_loop) v \<noteq> {}"
+                              by (simp add: h_NsP nonPRefsOf_def refsOf_def refs_F_CD_3WTs_loop 
                                 trancl_in)
                           next
-                            assume "v \<noteq> ''PrController_v1''"
-                            show "nonPRefsOf (toFr F_CD_3WTs) v \<noteq> {}"
-                            using h1 h2 h3 h4 h5 h6 h7 h8 h9 h10 
-                              by (auto simp add: h_NsP nonPRefsOf_def refsOf_def refs_F_CD_3WTs image_def)
+                            assume h11: "v \<noteq> ''PrController_v1''"
+                            show "nonPRefsOf (toFr F_CD_3WTs_loop) v \<noteq> {}"
+                            proof (case_tac "v = ''PrController_win''")
+                              assume "v = ''PrController_win''"
+                              then show "nonPRefsOf (toFr F_CD_3WTs_loop) v \<noteq> {}"
+                                by (simp add: h_NsP nonPRefsOf_def refsOf_def refs_F_CD_3WTs_loop 
+                                  trancl_in)
+                            next
+                              assume "v \<noteq> ''PrController_win''"
+                              then show "nonPRefsOf (toFr F_CD_3WTs_loop) v \<noteq> {}"
+                              using h1 h2 h3 h4 h5 h6 h7 h8 h9 h10 h1
+                                by (auto simp add: h_NsP nonPRefsOf_def refsOf_def 
+                                  refs_F_CD_3WTs_loop image_def)
+                            qed
                           qed
                         qed
                       qed
@@ -663,66 +692,71 @@ lemma wf_F_CD_3WTs: "is_wf_fr (toFr F_CD_3WTs)"
       qed
     next
       apply_end(rule conjI)
-      have h_wf_g: "is_wf_g (toSGr SG_CD_3WTs)"
-        using wf_SG_CD_3WTs
+      have h_wf_g: "is_wf_g (toSGr SG_CD_3WTs_loop)"
+        using wf_SG_CD_3WTs_loop
         by (simp add: is_wf_sg_def)
-      show "acyclic_fr (toFr F_CD_3WTs)"
+      show "acyclic_fr (toFr F_CD_3WTs_loop)"
       proof -
-          from wf_SG_CD_3WTs have "acyclic (inh (sg (toFr F_CD_3WTs)))"
-            by (simp add: is_wf_sg_def acyclicGr_def inh_def F_CD_3WTs_def toFr_def)
-          then show "acyclic_fr (toFr F_CD_3WTs)"
+          from wf_SG_CD_3WTs_loop have "acyclic (inh (sg (toFr F_CD_3WTs_loop)))"
+            by (simp add: is_wf_sg_def acyclicGr_def inh_def F_CD_3WTs_loop_def toFr_def)
+          then show "acyclic_fr (toFr F_CD_3WTs_loop)"
           proof (simp add: acyclic_fr_def)
-            assume h1: "acyclic (inh (sg (toFr F_CD_3WTs)))"
-            have h2: "is_wf_g (toSGr (sg_ls (F_CD_3WTs)))"
-              using wf_SG_CD_3WTs by (simp add: F_CD_3WTs_def is_wf_sg_def)
-            have h3: "Domain (inh (sg (toFr F_CD_3WTs))) \<inter> Domain (refs (toFr F_CD_3WTs)) = {}"
+            assume h1: "acyclic (inh (sg (toFr F_CD_3WTs_loop)))"
+            have h2: "is_wf_g (toSGr (sg_ls (F_CD_3WTs_loop)))"
+              using wf_SG_CD_3WTs_loop by (simp add: F_CD_3WTs_loop_def is_wf_sg_def)
+            have h3: "Domain (inh (sg (toFr F_CD_3WTs_loop))) \<inter> Domain (refs (toFr F_CD_3WTs_loop)) = {}"
               using h2 
-                by (simp add: refs_F_CD_3WTs)(simp add: toFr_def inh_eq_consInh, eval)
-            have h4: "Range (refs (toFr F_CD_3WTs)) \<inter> Domain (inh (sg (toFr F_CD_3WTs))) = {}"
-              using h2 by (simp add: refs_F_CD_3WTs)(simp add: toFr_def inh_eq_consInh, eval)
-            have h5: "acyclic(refs (toFr F_CD_3WTs))"
-              by (simp add: refs_F_CD_3WTs)(auto simp add: rtrancl_in acyclic_def)
-            from h1 h3 h4 h5 show "acyclic (inh (sg (toFr F_CD_3WTs)) \<union> refs (toFr F_CD_3WTs))"
+                by (simp add: refs_F_CD_3WTs_loop)(simp add: toFr_def inh_eq_consInh, eval)
+            have h4: "Range (refs (toFr F_CD_3WTs_loop)) \<inter> Domain (inh (sg (toFr F_CD_3WTs_loop))) = {}"
+              using h2 by (simp add: refs_F_CD_3WTs_loop)(simp add: toFr_def inh_eq_consInh, eval)
+            have h5: "acyclic(refs (toFr F_CD_3WTs_loop))"
+              by (simp add: refs_F_CD_3WTs_loop)(auto simp add: rtrancl_in acyclic_def)
+            from h1 h3 h4 h5 show "acyclic (inh (sg (toFr F_CD_3WTs_loop)) \<union> refs (toFr F_CD_3WTs_loop))"
               by (simp add: acyclic_Un)
           qed
         qed
     next
-      show "proxies_dont_inherit (toFr F_CD_3WTs)"
+      show "proxies_dont_inherit (toFr F_CD_3WTs_loop)"
       proof (simp add: proxies_dont_inherit_def, rule equalityI, rule subsetI)
         fix x
-        assume "x \<in> ran (src (sg (toFr F_CD_3WTs)) |` EsI (sg (toFr F_CD_3WTs))) \<inter>
-             NsP (sg (toFr F_CD_3WTs))"
+        assume "x \<in> ran (src (sg (toFr F_CD_3WTs_loop)) |` EsI (sg (toFr F_CD_3WTs_loop))) \<inter>
+             NsP (sg (toFr F_CD_3WTs_loop))"
         then show "x \<in> {}"
         by (simp add: h_NsP)(auto simp add: restrict_map_def 
-          F_CD_3WTs_def toFr_def vimage_def SG_CD_3WTs_def toSGr_def EsI_def EsTy_def ran_def
+          F_CD_3WTs_loop_def toFr_def vimage_def SG_CD_3WTs_loop_def toSGr_def EsI_def EsTy_def ran_def
           split: if_splits)
       next
-        show "{} \<subseteq> ran (src (sg (toFr F_CD_3WTs)) |` EsI (sg (toFr F_CD_3WTs))) \<inter> NsP (sg (toFr F_CD_3WTs))"
+        show "{} \<subseteq> ran (src (sg (toFr F_CD_3WTs_loop)) |` EsI (sg (toFr F_CD_3WTs_loop))) \<inter> NsP (sg (toFr F_CD_3WTs_loop))"
         by (simp)
       qed
     qed
   qed
 
-definition T_F_ASD_3WTs :: "MorphL"
+definition T_F_ASD_3WTs_loop :: "MorphL"
 where
-   "T_F_ASD_3WTs \<equiv> \<lparr>fVL = [(''WaterTanksASD'', ''ASD''), 
+   "T_F_ASD_3WTs_loop \<equiv> \<lparr>fVL = [(''WaterTanksASD'', ''ASD''), 
    (''WaterTanksSys'', ''System''), 
    (''CompWaterTanksSys1'', ''Composition''),
    (''CompWaterTanksSys2'', ''Composition''), 
    (''CompWaterTanksSys3'', ''Composition''),
    (''TanksControl1'', ''EComponent''), 
-   (''TanksControl2'', ''EComponent''),
+   (''TanksControl2'', ''EComponent''), 
    (''CompTanksControl1Valve'', ''Composition''),
-   (''CompTanksControl1WaterTank'', ''Composition''),
+   (''CompTanksControl1WaterTank'', ''Composition''), 
    (''CompTanksControl2WaterTank'', ''Composition''),
    (''Controller'', ''EComponent''),
    (''Valve'', ''POComponent''), 
-   (''WaterTank'', ''POComponent''),
-   (''FlowRate'', ''DType''), (''Area'', ''DType''), 
-   (''Height'', ''DType''), (''OpenClosed'', ''Enumeration''),
-   (''WaterTank_win'', ''FlowPort''), (''WaterTank_wout'', ''FlowPort''), 
-   (''Valve_v2'', ''FlowPort''), (''Valve_w'', ''FlowPort''), 
-   (''Controller_v1'', ''FlowPort'')], 
+   (''WaterTank'', ''POComponent''), 
+   (''FlowRate'', ''DType''), 
+   (''Area'', ''DType''), 
+   (''Height'', ''DType''), 
+   (''OpenClosed'', ''Enumeration''), 
+   (''WaterTank_win'', ''FlowPort''), 
+   (''WaterTank_wout'', ''FlowPort''), 
+   (''Valve_v2'', ''FlowPort''), 
+   (''Valve_w'', ''FlowPort''), 
+   (''Controller_v1'', ''FlowPort''), 
+   (''Controller_win'', ''FlowPort'')], 
     fEL = [
       (''EWaterTanksASD_WaterTanksSys'', ''Eblocks''), 
       (''EWaterTanksASD_TanksControl1'', ''Eblocks''), 
@@ -749,14 +783,16 @@ where
       (''E_WaterTank_out'', ''EBlockProps''), 
       (''E_Valve_v2'', ''EBlockProps''), 
       (''E_Valve_w'', ''EBlockProps''), 
-      (''E_Controller_v1'', ''EBlockProps''),
+      (''E_Controller_v1'', ''EBlockProps''), 
+      (''E_Controller_win'', ''EBlockProps''),
       (''E_Dep_w_v2'', ''EFlowPortDepends''), 
-      (''E_Dep_wout_win'', ''EFlowPortDepends'')]\<rparr>"
+      (''E_Dep_wout_win'', ''EFlowPortDepends''),
+      (''E_Dep_v1_win'', ''EFlowPortDepends'')]\<rparr>"
 
 (*Define the other morphism*)
-definition T_F_CD_3WTs :: "MorphL"
+definition T_F_CD_3WTs_loop :: "MorphL"
 where
-   "T_F_CD_3WTs \<equiv> \<lparr>fVL = [(''PrWaterTank'', ''PrBlock3''), 
+   "T_F_CD_3WTs_loop \<equiv> \<lparr>fVL = [(''PrWaterTank'', ''PrBlock3''), 
       (''PrValve'', ''PrBlock3''), 
       (''PrTanksControl1'', ''PrBlock3''), 
       (''PrTanksControl2'', ''PrBlock3''), 
@@ -773,37 +809,41 @@ where
       (''C_w_win1'', ''Connector''), 
       (''C_wout1_win2'', ''Connector''), 
       (''C_wout2_win3'', ''Connector''),
-      (''C_v1_v2'', ''Connector''),
-      (''v1'', ''Port''), (''v2'', ''Port''), 
-      (''w'', ''Port''), (''win1'', ''Port''), 
-      (''wout1'', ''Port''), (''win2'', ''Port''), 
+      (''C_v1_v2'', ''Connector''), 
+      (''C_wout3_win'', ''Connector''),
+      (''v1'', ''Port''), (''win'', ''Port''), 
+      (''v2'', ''Port''), (''w'', ''Port''), 
+      (''win1'', ''Port''), 
+      (''wout1'', ''Port''), 
+      (''win2'', ''Port''), 
       (''wout2'', ''Port''),
       (''win3'', ''Port''), (''wout3'', ''Port''), 
       (''PrValve_v2'', ''PrFlowPort2''), 
       (''PrValve_w'', ''PrFlowPort2''), 
       (''PrWaterTank_win'', ''PrFlowPort2''), 
       (''PrWaterTank_wout'', ''PrFlowPort2''), 
-      (''PrController_v1'', ''PrFlowPort2'')],
+      (''PrController_v1'', ''PrFlowPort2''),
+      (''PrController_win'', ''PrFlowPort2'')],
     fEL = [(''ECD_WTSys'', ''ECDblocks''), (''ECD_V'', ''ECDblocks''), 
       (''ECD_WT1'', ''ECDblocks''), (''ECD_WT2'', ''ECDblocks''),
       (''ECD_WT3'', ''ECDblocks''), (''ECD_C'', ''ECDblocks''),
       (''ECD_TC1'', ''ECDblocks''), (''ECD_TC2'', ''ECDblocks''),
       (''ECD_C_v1_v2'', ''ECDconnectors''), (''ECD_C_w_win1'', ''ECDconnectors''),
       (''ECD_C_wout1_win2'', ''ECDconnectors''), 
-      (''ECD_C_wout2_win3'', ''ECDconnectors''),
+      (''ECD_C_wout2_win3'', ''ECDconnectors''), 
       (''E_C_v1_v2_src'', ''EC_src''), (''E_C_v1_v2_tgt'', ''EC_tgt''), 
       (''E_C_w_win1_src'', ''EC_src''), (''E_C_w_win1_tgt'', ''EC_tgt''), 
       (''E_C_wout1_win2_src'', ''EC_src''), (''E_C_wout1_win2_tgt'', ''EC_tgt''), 
-      (''E_C_wout2_win3_src'', ''EC_src''), (''E_C_wout2_win3_tgt'', ''EC_tgt''), 
-      (''E_C_v1'', ''EBIports''), (''E_V_v2'', ''EBIports''),   
-      (''E_V_w'', ''EBIports''), 
+      (''E_C_wout2_win3_src'', ''EC_src''), (''E_C_wout2_win3_tgt'', ''EC_tgt''),
+      (''E_C_wout3_win_src'', ''EC_src''), (''E_C_wout3_win_tgt'', ''EC_tgt''),
+      (''E_C_v1'', ''EBIports''), (''E_C_win'', ''EBIports''), 
+      (''E_V_v2'', ''EBIports''), (''E_V_w'', ''EBIports''), 
       (''E_WT1_win1'', ''EBIports''),
-      (''E_WT1_wout1'', ''EBIports''), 
-      (''E_WT2_win2'', ''EBIports''),
-      (''E_WT2_wout2'', ''EBIports''), 
-      (''E_WT3_win3'', ''EBIports''), 
+      (''E_WT1_wout1'', ''EBIports''), (''E_WT2_win2'', ''EBIports''),
+      (''E_WT2_wout2'', ''EBIports''), (''E_WT3_win3'', ''EBIports''), 
       (''E_WT3_wout3'', ''EBIports''), (''E_v1_ty'', ''EPortType''), 
-      (''E_v2_ty'', ''EPortType''), (''E_w_ty'', ''EPortType''),
+      (''E_v2_ty'', ''EPortType''), (''E_win_ty'', ''EPortType''), 
+      (''E_w_ty'', ''EPortType''),
       (''E_win1_ty'', ''EPortType''), 
       (''E_wout1_ty'', ''EPortType''),
       (''E_win2_ty'', ''EPortType''), (''E_wout2_ty'', ''EPortType''), 
@@ -816,196 +856,192 @@ where
       (''ERPrValve_w'', ''ERPrFlowPort2''), 
       (''ERPrWaterTank_win'', ''ERPrFlowPort2''),
       (''ERPrWaterTank_wout'', ''ERPrFlowPort2''), 
-      (''ERPrController_v1'', ''ERPrFlowPort2'')]\<rparr>"
+      (''ERPrController_v1'', ''ERPrFlowPort2''),
+      (''ERPrController_win'', ''ERPrFlowPort2'')]\<rparr>"
 
-definition GFG_3WTs :: "GFGr_ls"
+definition GFG_3WTs_loop :: "GFGr_ls"
 where
-  "GFG_3WTs \<equiv> 
-    \<lparr>NsG = [''F_ASD_3WTs'', ''F_CD_3WTs''], 
+  "GFG_3WTs_loop \<equiv> 
+    \<lparr>NsG = [''F_ASD_3WTs_loop'', ''F_CD_3WTs_loop''], 
       EsG= [''E_F_CD_3WTs_ASD'', ''E_F_ASD_3WTs'', ''E_F_CD_3WTs''], 
-      srcG = [(''E_F_CD_3WTs_ASD'', ''F_CD_3WTs''), 
-        (''E_F_ASD_3WTs'', ''F_ASD_3WTs''),
-        (''E_F_CD_3WTs'', ''F_CD_3WTs'')],
-      tgtG = [(''E_F_CD_3WTs_ASD'', ''F_ASD_3WTs''), 
-        (''E_F_ASD_3WTs'', ''F_ASD_3WTs''),
-        (''E_F_CD_3WTs'', ''F_CD_3WTs'')],
+      srcG = [(''E_F_CD_3WTs_ASD'', ''F_CD_3WTs_loop''), 
+        (''E_F_ASD_3WTs'', ''F_ASD_3WTs_loop''),
+        (''E_F_CD_3WTs'', ''F_CD_3WTs_loop'')],
+      tgtG = [(''E_F_CD_3WTs_ASD'', ''F_ASD_3WTs_loop''), 
+        (''E_F_ASD_3WTs'', ''F_ASD_3WTs_loop''),
+        (''E_F_CD_3WTs'', ''F_CD_3WTs_loop'')],
       ext_ty_ls = [(''E_F_CD_3WTs_ASD'', eimp), (''E_F_ASD_3WTs'', eimp),
         (''E_F_CD_3WTs'', eimp)]\<rparr>"
 
 axiomatization
 where
-  Es_GFG_3WTs: "Es (toGFGr(GFG_3WTs)) \<subseteq> E_A"
-  and Ns_GFG_3WTs: "Ns (toGFGr(GFG_3WTs)) \<subseteq> V_A"
+  Es_GFG_3WTs_loop: "Es (toGFGr(GFG_3WTs_loop)) \<subseteq> E_A"
+  and Ns_GFG_3WTs_loop: "Ns (toGFGr(GFG_3WTs_loop)) \<subseteq> V_A"
 
-lemma is_wf_GFG_3WTs: "is_wf_gfg_ls GFG_3WTs"
+lemma is_wf_GFG_3WTs_loop: "is_wf_gfg_ls GFG_3WTs_loop"
   proof -
-    have h_wf_g: "is_wf_g (toGFGr GFG_3WTs)"
-      using Es_GFG_3WTs Ns_GFG_3WTs
-        by (auto simp add: is_wf_g_def GFG_3WTs_def ftotal_on_def toGFGr_def)
+    have h_wf_g: "is_wf_g (toGFGr GFG_3WTs_loop)"
+      using Es_GFG_3WTs_loop Ns_GFG_3WTs_loop
+        by (auto simp add: is_wf_g_def GFG_3WTs_loop_def ftotal_on_def toGFGr_def)
     show ?thesis
     proof (simp add: is_wf_gfg_ls_def, rule conjI)
-      show "distinct (NsG GFG_3WTs)"
-      by (simp add: GFG_3WTs_def)
+      show "distinct (NsG GFG_3WTs_loop)"
+      by (simp add: GFG_3WTs_loop_def)
     next
-      apply_end(rule conjI)
-      show "distinct (map fst (srcG GFG_3WTs))"
-        by (simp add: GFG_3WTs_def)
+      apply_end (rule conjI)
+      show "distinct (map fst (srcG GFG_3WTs_loop))"
+        by (simp add: GFG_3WTs_loop_def)
     next
-      apply_end(rule conjI)
-      show "distinct (map fst (tgtG GFG_3WTs))"
-        by (simp add: GFG_3WTs_def)
+      apply_end (rule conjI)
+      show "distinct (map fst (tgtG GFG_3WTs_loop))"
+        by (simp add: GFG_3WTs_loop_def)
     next
-      show "is_wf_gfg (toGFGr GFG_3WTs)"
+      show "is_wf_gfg (toGFGr GFG_3WTs_loop)"
         proof (simp add: is_wf_gfg_def, rule conjI)
-          show "is_wf_g (toGFGr GFG_3WTs)"
+          show "is_wf_g (toGFGr GFG_3WTs_loop)"
             using h_wf_g by simp
         next
           apply_end (rule conjI)
-          show "ftotal_on (ext_ty (toGFGr GFG_3WTs)) (Es (toGFGr GFG_3WTs)) GFGEdgeTy_set"
-            by (simp add: GFG_3WTs_def toGFGr_def GFGEdgeTy_set_def ftotal_on_def)
+          show "ftotal_on (ext_ty (toGFGr GFG_3WTs_loop)) (Es (toGFGr GFG_3WTs_loop)) GFGEdgeTy_set"
+            by (simp add: GFG_3WTs_loop_def toGFGr_def GFGEdgeTy_set_def ftotal_on_def)
         next
           apply_end (rule conjI)
-          show "NodesWithSelfEdges (toGFGr GFG_3WTs)"
+          show "NodesWithSelfEdges (toGFGr GFG_3WTs_loop)"
           proof (simp add: NodesWithSelfEdges_def, clarify)
             fix v
-            assume "v \<in> Ns (toGFGr GFG_3WTs)"
-            then have h1: "v = ''F_CD_3WTs'' \<or> v = ''F_ASD_3WTs''"
-              by (auto simp add: GFG_3WTs_def toGFGr_def)
-            then show "\<exists>e. e \<in> Es (toGFGr GFG_3WTs) 
-              \<and> src (toGFGr GFG_3WTs) e = Some v 
-              \<and> tgt (toGFGr GFG_3WTs) e = Some v"
-            by (simp add:  GFG_3WTs_def toGFGr_def NodesWithSelfEdges_def)
+            assume "v \<in> Ns (toGFGr GFG_3WTs_loop)"
+            then have h1: "v = ''F_CD_3WTs_loop'' \<or> v = ''F_ASD_3WTs_loop''"
+              by (auto simp add: GFG_3WTs_loop_def toGFGr_def)
+            then show "\<exists>e. e \<in> Es (toGFGr GFG_3WTs_loop) 
+              \<and> src (toGFGr GFG_3WTs_loop) e = Some v 
+              \<and> tgt (toGFGr GFG_3WTs_loop) e = Some v"
+            by (simp add:  GFG_3WTs_loop_def toGFGr_def NodesWithSelfEdges_def)
               (erule disjE, rule exI[where x= "''E_F_CD_3WTs''"], simp_all, 
                 rule exI[where x= "''E_F_ASD_3WTs''"], simp)
           qed
         next
           show "acyclicGr
-            (restrict (toGFGr GFG_3WTs)
-              (Es (toGFGr GFG_3WTs) - EsId (toGFGr GFG_3WTs)))"
-          by (auto simp add: GFG_3WTs_def toGFGr_def EsId_def restrict_def acyclicGr_def
+            (restrict (toGFGr GFG_3WTs_loop)
+              (Es (toGFGr GFG_3WTs_loop) - EsId (toGFGr GFG_3WTs_loop)))"
+          by (auto simp add: GFG_3WTs_loop_def toGFGr_def EsId_def restrict_def acyclicGr_def
             relOfGr_def rst_Ns_def rst_fun_def adjacent_def acyclic_def elim: tranclE)
      qed
    qed
   qed
 
-definition Mdl_3WTs :: "Mdl_ls"
+definition Mdl_3WTs_loop :: "Mdl_ls"
 where
-  "Mdl_3WTs \<equiv> \<lparr>gfgL = GFG_3WTs, 
-    frdL = [(''F_ASD_3WTs'', F_ASD_3WTs), (''F_CD_3WTs'', F_CD_3WTs)]\<rparr>"
+  "Mdl_3WTs_loop \<equiv> \<lparr>gfgL = GFG_3WTs_loop, 
+    frdL = [(''F_ASD_3WTs_loop'', F_ASD_3WTs_loop), (''F_CD_3WTs_loop'', F_CD_3WTs_loop)]\<rparr>"
 
-lemma is_wf_mdl_3WTs: "is_wf_mdl (toMdl Mdl_3WTs)"
+lemma is_wf_mdl_3WTs_loop: "is_wf_mdl (toMdl Mdl_3WTs_loop)"
   proof (simp add: is_wf_mdl_def, rule conjI)
-    show "\<forall>F. F \<in> ran (frd (toMdl Mdl_3WTs)) \<longrightarrow> is_wf_fr F"
+    show "\<forall>F. F \<in> ran (frd (toMdl Mdl_3WTs_loop)) \<longrightarrow> is_wf_fr F"
     proof (clarify)
       fix F
-      assume "F \<in> ran (frd (toMdl Mdl_3WTs))"
-      then have h1: "F = (toFr F_ASD_3WTs) \<or> F = (toFr F_CD_3WTs)"
-        by (auto simp add: INTO_SysML_MM_def toMdl_def Mdl_3WTs_def)
+      assume "F \<in> ran (frd (toMdl Mdl_3WTs_loop))"
+      then have h1: "F = (toFr F_ASD_3WTs_loop) \<or> F = (toFr F_CD_3WTs_loop)"
+        by (auto simp add: INTO_SysML_MM_def toMdl_def Mdl_3WTs_loop_def)
       then show "is_wf_fr F"
-      proof (case_tac "F = toFr F_ASD_3WTs")
-        assume "F = toFr F_ASD_3WTs"
+      proof (case_tac "F = toFr F_ASD_3WTs_loop")
+        assume "F = toFr F_ASD_3WTs_loop"
         then show "is_wf_fr F"
-          by (simp add: wf_F_ASD_3WTs)
+          by (simp add: wf_F_ASD_3WTs_loop)
       next
-        assume h2: "F \<noteq> toFr F_ASD_3WTs"
+        assume h2: "F \<noteq> toFr F_ASD_3WTs_loop"
         then show "is_wf_fr F"
-        proof (case_tac "F = toFr F_CD_3WTs")
-          assume "F = toFr F_CD_3WTs"
+        proof (case_tac "F = toFr F_CD_3WTs_loop")
+          assume "F = toFr F_CD_3WTs_loop"
           then show "is_wf_fr F"
-            by (simp add: wf_F_CD_3WTs)
+            by (simp add: wf_F_CD_3WTs_loop)
         next
-          assume h3: "F \<noteq> toFr F_CD_3WTs"
+          assume h3: "F \<noteq> toFr F_CD_3WTs_loop"
           then show "is_wf_fr F" using h1 h2 by (simp)
         qed
       qed
     qed
   next
     apply_end(rule conjI)
-    show "is_wf_gfg_ls (gfg (toMdl Mdl_3WTs))"
-      by (simp add: is_wf_GFG_3WTs Mdl_3WTs_def toMdl_def)
+    show "is_wf_gfg_ls (gfg (toMdl Mdl_3WTs_loop))"
+      by (simp add: is_wf_GFG_3WTs_loop Mdl_3WTs_loop_def toMdl_def)
   next
     apply_end(rule conjI)
-    show "ftotal_on (frd (toMdl Mdl_3WTs)) (set (NsG (gfg (toMdl Mdl_3WTs)))) fr_set"
-      by (simp add: ftotal_on_def Mdl_3WTs_def toMdl_def GFG_3WTs_def F_ASD_3WTs_def
-        toFr_def toSGr_def SG_ASD_3WTs_def F_CD_3WTs_def fr_set_def is_fr_def)
+    show "ftotal_on (frd (toMdl Mdl_3WTs_loop)) (set (NsG (gfg (toMdl Mdl_3WTs_loop)))) fr_set"
+      by (simp add: ftotal_on_def Mdl_3WTs_loop_def toMdl_def GFG_3WTs_loop_def F_ASD_3WTs_loop_def
+        toFr_def toSGr_def SG_ASD_3WTs_loop_def F_CD_3WTs_loop_def fr_set_def is_fr_def)
   next
     apply_end(rule conjI)
-    show "disjMdlFrs (toMdl Mdl_3WTs)"
-      by (simp add: disjMdlFrs_def Mdl_3WTs_def disjFs_def disjGsL_def 
-        GFG_3WTs_def F_Common_def SG_F_Common_def F_Props_def SG_F_Props_def
-        toFr_def toMdl_def toSGr_def SG_ASD_3WTs_def SG_CD_3WTs_def
-        F_ASD_3WTs_def F_CD_3WTs_def)
+    show "disjMdlFrs (toMdl Mdl_3WTs_loop)"
+      by (simp add: disjMdlFrs_def Mdl_3WTs_loop_def disjFs_def disjGsL_def 
+        GFG_3WTs_loop_def F_Common_def SG_F_Common_def F_Props_def SG_F_Props_def
+        toFr_def toMdl_def toSGr_def SG_ASD_3WTs_loop_def SG_CD_3WTs_loop_def
+        F_ASD_3WTs_loop_def F_CD_3WTs_loop_def)
   next
-    show "mUM2GFG (toMdl Mdl_3WTs)
-      \<in> morphF2GFGr (UMdlFs (toMdl Mdl_3WTs)) (toGFGr (gfg (toMdl Mdl_3WTs)))"
-      by (simp add: UGM_eq_ConsUGM)
+    show "mUM2GFG (toMdl Mdl_3WTs_loop)
+      \<in> morphF2GFGr (UMdlFs (toMdl Mdl_3WTs_loop)) (toGFGr (gfg (toMdl Mdl_3WTs_loop)))"
+      by (simp)
   qed
 
-definition MdlTy_3WTs :: "MdlTy_ls"
+definition MdlTy_3WTs_loop :: "MdlTy_ls"
 where
-  "MdlTy_3WTs \<equiv> \<lparr>tmdlL = INTO_SysML_MM_T, 
-    mdlL = Mdl_3WTs,
-    mtyL = (consUGM T_F_ASD_3WTs T_F_CD_3WTs)\<rparr>"
+  "MdlTy_3WTs_loop \<equiv> \<lparr>tmdlL = INTO_SysML_MM_T, 
+    mdlL = Mdl_3WTs_loop,
+    mtyL = (consUGM T_F_ASD_3WTs_loop T_F_CD_3WTs_loop)\<rparr>"
 
-lemma is_wf_mdlt_3WTs: "is_wf_mdlty (toMdlTy MdlTy_3WTs)"
+lemma is_wf_mdlt_3WTs: "is_wf_mdlty (toMdlTy MdlTy_3WTs_loop)"
   proof (simp add: is_wf_mdlty_def, rule conjI)
-    show "is_wf_tmdl (tmdl (toMdlTy MdlTy_3WTs))"
-      by (simp add: is_wf_INTO_SysML_MM_T MdlTy_3WTs_def toMdlTy_def)
+    show "is_wf_tmdl (tmdl (toMdlTy MdlTy_3WTs_loop))"
+      by (simp add: is_wf_INTO_SysML_MM_T MdlTy_3WTs_loop_def toMdlTy_def)
   next
     apply_end(rule conjI)
-    show "is_wf_mdl (mdl (toMdlTy MdlTy_3WTs))"
-      by (simp add: is_wf_mdl_3WTs toMdlTy_def MdlTy_3WTs_def)
+    show "is_wf_mdl (mdl (toMdlTy MdlTy_3WTs_loop))"
+      by (simp add: is_wf_mdl_3WTs_loop toMdlTy_def MdlTy_3WTs_loop_def)
   next
-    show "mty (toMdlTy MdlTy_3WTs)
-    \<in> morphFr (UMdlFs (mdl (toMdlTy MdlTy_3WTs))) (fr (UTyMdlFs (tmdl (toMdlTy MdlTy_3WTs))))"
-    by (simp add: toMdlTy_def MdlTy_3WTs_def)
+    show "mty (toMdlTy MdlTy_3WTs_loop)
+    \<in> morphFr (UMdlFs (mdl (toMdlTy MdlTy_3WTs_loop))) (fr (UTyMdlFs (tmdl (toMdlTy MdlTy_3WTs_loop))))"
+    by (simp add: toMdlTy_def MdlTy_3WTs_loop_def)
   qed
 
-value "consUMdlFs (mdlL MdlTy_3WTs)"
+value "consUMdlFs (mdlL MdlTy_3WTs_loop)"
  
-value "INTO_SysML_toPDG_Nodes (mdlL MdlTy_3WTs) (toMorph (mtyL MdlTy_3WTs))"
+value "INTO_SysML_toPDG_Nodes (mdlL MdlTy_3WTs_loop) (toMorph (mtyL MdlTy_3WTs_loop))"
 
-value "INTO_SysML_toPDG (mdlL MdlTy_3WTs) (toMorph (mtyL MdlTy_3WTs))"
+value "INTO_SysML_toPDG MdlTy_3WTs_loop"
 
 fun portNodes :: "Mdl_ls \<Rightarrow> Morph \<Rightarrow> V list"
 where
    "portNodes ML m = 
-    (filter (\<lambda>v . (fV m) v = Some ''Port'' )((NsG o sg_ls) (consUMdlFs ML)))"
+    (filter (\<lambda>v . (fV m) v = Some ''Connector'' )((NsG o sg_ls) (consUMdlFs ML)))"
 
 fun edgesOfTy :: "Mdl_ls \<Rightarrow> Morph \<Rightarrow> E \<Rightarrow>E list"
 where
    "edgesOfTy ML m e = 
     (filter (\<lambda>v . (fE m) v = Some e )((EsG o sg_ls) (consUMdlFs ML)))"
 
-value "portNodes (mdlL MdlTy_3WTs) (toMorph (mtyL MdlTy_3WTs))"
+value "portNodes (mdlL MdlTy_3WTs_loop) (toMorph (mtyL MdlTy_3WTs_loop))"
 
-value "edgesOfTy (mdlL MdlTy_3WTs) (toMorph (mtyL MdlTy_3WTs)) ''EPortType''"
+value "edgesOfTy (mdlL MdlTy_3WTs_loop) (toMorph  (mtyL MdlTy_3WTs_loop)) ''EPortType''"
 
-value "edgesOfTy (mdlL MdlTy_3WTs) (toMorph (mtyL MdlTy_3WTs)) ''EFlowPortDepends''"
+value "edgesOfTy (mdlL MdlTy_3WTs_loop) (toMorph  (mtyL MdlTy_3WTs_loop)) ''EFlowPortDepends''"
 
-value "edgesOfTy (mdlL MdlTy_3WTs) (toMorph (mtyL MdlTy_3WTs)) ''EBIports''"
+value "edgesOfTy (mdlL MdlTy_3WTs_loop) (toMorph (mtyL MdlTy_3WTs_loop)) ''EBIports''"
 
-value "the (tgt (sg (toFr (consUMdlFs (mdlL MdlTy_3WTs)))) ''E_WT3_win3'')"
+value "the (tgt (sg (toFr (consUMdlFs (mdlL MdlTy_3WTs_loop)))) ''E_WT3_win3'')"
 
-value "the (tgt (sg (toFr (consUMdlFs (mdlL MdlTy_3WTs)))) ''E_v2_ty'')"
+value "the (tgt (sg (toFr (consUMdlFs (mdlL MdlTy_3WTs_loop)))) ''E_v2_ty'')"
 
-value "(set (consSrcStF (consUMdlFs (mdlL MdlTy_3WTs)))) ``{''E_Dep_w_v2''}"
+value "(set (consSrcStF (consUMdlFs (mdlL MdlTy_3WTs_loop)))) ``{''E_Dep_v1_win''}"
 
-value "the (tgt (sg (toFr (consUMdlFs (mdlL MdlTy_3WTs)))) ''E_Dep_w_v2'')"
+value "the (tgt (sg (toFr (consUMdlFs (mdlL MdlTy_3WTs_loop)))) ''E_Dep_v1_win'')"
 
 (*Get these functions right*)
-value "getBlockInstanceOfPort (toMorph (mtyL MdlTy_3WTs)) (consUMdlFs (mdlL MdlTy_3WTs)) ''win3''"
-value "getOtherInternalPorts (toMorph (mtyL MdlTy_3WTs)) (consUMdlFs (mdlL MdlTy_3WTs)) ''win3''"
-value "getFlowPortTypeOfPort (toMorph (mtyL MdlTy_3WTs)) (consUMdlFs (mdlL MdlTy_3WTs)) ''win3''"
+value "getBlockInstanceOfPort (toMorph (mtyL MdlTy_3WTs_loop)) (consUMdlFs (mdlL MdlTy_3WTs_loop)) ''win''"
+value "getOtherInternalPorts (toMorph (mtyL MdlTy_3WTs_loop)) (consUMdlFs (mdlL MdlTy_3WTs_loop)) ''win''"
+value "getFlowPortTypeOfPort (toMorph (mtyL MdlTy_3WTs_loop)) (consUMdlFs (mdlL MdlTy_3WTs_loop)) ''win''"
 
-(*
-value "getDependentPortOfV (mty_ls MdlTy_3WTs) (consUMdlFs (mdl_ls MdlTy_3WTs)) ''w'' ''PrValve_v2''"
-*)
-value "(fV (toMorph (mtyL MdlTy_3WTs))) (the (tgt (sg (toFr (consUMdlFs (mdlL MdlTy_3WTs)))) ''E_v2_ty''))"
+value "(set(consTgtStF (consUMdlFs (mdlL MdlTy_3WTs_loop)))) ``{''E_v2_ty''}"
 
-value "(set(consTgtStF (consUMdlFs (mdlL MdlTy_3WTs)))) ``{''E_v2_ty''}"
-
-value "consClanF ''PrController_v1'' (consUMdlFs (mdlL MdlTy_3WTs))"
+value "consClanF ''PrController_v1'' (consUMdlFs (mdlL MdlTy_3WTs_loop))"
 
 fun internalConnectionsOf :: "Mdl_ls \<Rightarrow> Morph \<Rightarrow> V \<Rightarrow> Gr_ls"
 where
@@ -1018,8 +1054,8 @@ where
     (filter (\<lambda> e. (getFlowPortTypeOfPort m (consUMdlFs ML) v) \<in> (set (consSrcStF (consUMdlFs ML))) ``{e})
             (filter (\<lambda> e. (fE m) e = Some ''EFlowPortDepends'') (EsG (sg_ls (consUMdlFs ML)))))"
 
-value "buildGrForConnector (toMorph (mtyL MdlTy_3WTs)) (consUMdlFs (mdlL MdlTy_3WTs)) ''C_w_win1''"
-value "dependsGrOf (mdlL MdlTy_3WTs) (toMorph (mtyL MdlTy_3WTs)) ''win3''"
-value "internalConnectionsOf (mdlL MdlTy_3WTs) (toMorph (mtyL MdlTy_3WTs)) ''w''"
+value "buildGrForConnector (toMorph (mtyL MdlTy_3WTs_loop)) (consUMdlFs (mdlL MdlTy_3WTs_loop)) ''C_v1_v2''"
+value "dependsGrOf (mdlL MdlTy_3WTs_loop) (toMorph (mtyL MdlTy_3WTs_loop)) ''v1''"
+value "internalConnectionsOf (mdlL MdlTy_3WTs_loop) (toMorph (mtyL MdlTy_3WTs_loop)) ''win''"
 
 end
